Finished lemma2 and lemma5, rewrote lemma1, lots of extra lemmas

matching-logic/src/Experimental/Unification.v
@@ -13,7 +13,7 @@ From Coq.Unicode Require Import Utf8.
 From Coq.micromega Require Import Lia.
 
 From MatchingLogic Require Import Logic ProofMode.MLPM.
-From MatchingLogic.Theories Require Import Definedness_Syntax Definedness_ProofSystem FOEquality_ProofSystem.
+From MatchingLogic.Theories Require Import Definedness_Syntax Definedness_ProofSystem FOEquality_ProofSystem DeductionTheorem.
 From MatchingLogic.Utils Require Import stdpp_ext.
 
 Require Import MatchingLogic.wftactics.
@@ -214,7 +214,8 @@ Section ProofSystemTheorems.
     cbn. rewrite mu_free_bevar_subst; wf_auto2.
   Defined.
 
-  Lemma Lemma₂ : forall Γ φ x φ',
+  (* Since this isn't very useful for multi version, maybe delete? *)
+  Lemma Lemma₂_single : forall Γ φ x φ',
     theory ⊆ Γ -> well_formed φ -> mu_free φ -> well_formed φ' ->
     Γ ⊢ is_functional φ ->
     Γ ⊢ φ^[[evar: x ↦ φ']] and patt_free_evar x =ml φ' --->
@@ -237,17 +238,100 @@ Section ProofSystemTheorems.
     mlExact "H2".
   Defined.
 
+  (* stdpp_ext *)
+  Lemma fold_left_preserves_function {A : Type} (t : A -> Pattern) (P : Pattern -> Prop) (f : Pattern -> A -> Pattern) x xs :
+    P x -> foldr (fun c a => P (t c) /\ a) True xs -> (forall a b, P a -> P (t b) -> P (f a b)) -> P (fold_left f xs x).
+  Proof.
+    intros px pxs ppf.
+    revert x px.
+    induction xs; intros.
+    exact px.
+    simpl in pxs.
+    destruct pxs.
+    apply IHxs.
+    exact H0.
+    apply ppf.
+    exact px.
+    exact H.
+  Defined.
+
+  Lemma foldr_preserves_function {A : Type} (t : A -> Pattern) (P : Pattern -> Prop) (f : A -> Pattern -> Pattern) x xs :
+    P x -> foldr (fun c a => P (t c) /\ a) True xs -> (forall a b, P a -> P (t b) -> P (f b a)) -> P (foldr f x xs).
+  Proof.
+    intros px pxs ppf.
+    revert x px.
+    induction xs; intros.
+    exact px.
+    simpl in pxs.
+    destruct pxs.
+    simpl.
+    apply ppf.
+    apply IHxs.
+    exact H0.
+    exact px.
+    exact H.
+  Defined.
+
+  Lemma foldr_preserves_function_set {A : Type} (t : A -> Pattern) (P : Pattern -> Set) (f : A -> Pattern -> Pattern) x xs :
+    P x -> foldr (fun c a => (P (t c) * a)%type) True xs -> (forall a b, P a -> P (t b) -> P (f b a)) -> P (foldr f x xs).
+  Proof.
+    intros px pxs ppf.
+    revert x px.
+    induction xs; intros.
+    exact px.
+    simpl in pxs.
+    destruct pxs.
+    simpl.
+    apply ppf.
+    apply IHxs.
+    exact f0.
+    exact px.
+    exact p.
+  Defined.
+
+  Lemma foldr_andb_equiv_foldr_conj {A : Type} (t : A -> bool) (xs : list A) : foldr (fun c a => t c && a) true xs <-> foldr (fun c a => (t c) = true /\ a) True xs.
+  Proof.
+    induction xs; simpl.
+    split; split.
+    destruct IHxs.
+    split; intro.
+    apply andb_true_iff in H1. destruct H1.
+    split. exact H1.
+    exact (H H2).
+    destruct H1.
+    apply andb_true_iff.
+    split.
+    exact H1.
+    exact (H0 H2).
+  Defined.
+
+  Lemma foldr_map_thing {A B C : Type} (f : A -> B -> B) (g : C -> A) (x : B) (xs : list C) : foldr f x (map g xs) = foldr (fun c a => f (g c) a) x xs.
+  Proof.
+    induction xs.
+    reflexivity.
+    simpl. f_equal. exact IHxs.
+  Defined.
+
+  (* pattern.v *)
   Lemma wf_fold_left {A : Type} (f : Pattern -> A -> Pattern) (t : A -> Pattern) x xs :
     well_formed x ->
     wf (map t xs) ->
     (forall a b, well_formed a -> well_formed (t b) -> well_formed (f a b)) ->
     well_formed (fold_left f xs x).
   Proof.
+    (* intros wfx wfxs wfpf. *)
+    (* revert x wfx. *)
+    (* induction xs; simpl. *)
+    (* intro. exact id. *)
+    (* intros. apply IHxs, wfpf; wf_auto2. *)
+  (* Restart. *)
     intros wfx wfxs wfpf.
-    revert x wfx.
-    induction xs; simpl.
-    intro. exact id.
-    intros. apply IHxs, wfpf; wf_auto2.
+    pose proof (fold_left_preserves_function t well_formed f x xs wfx).
+    simpl in H.
+    ospecialize* H.
+    apply foldr_andb_equiv_foldr_conj. unfold wf in wfxs. rewrite ! foldr_map_thing in wfxs. exact wfxs.
+    exact wfpf.
+    exact H.
   Defined.
 
   Lemma wf_foldr {A : Type} (f : A -> Pattern -> Pattern) (t : A -> Pattern) x xs :
@@ -256,47 +340,80 @@ Section ProofSystemTheorems.
     (forall a b, well_formed a -> well_formed (t b) -> well_formed (f b a)) ->
     well_formed (foldr f x xs).
   Proof.
+    (* intros wfx wfxs wfpf. *)
+    (* revert x wfx. *)
+    (* induction xs; simpl. *)
+    (* intro. exact id. *)
+    (* intros. apply wfpf; [apply IHxs |]; wf_auto2. *)
+  (* Restart. *)
     intros wfx wfxs wfpf.
-    revert x wfx.
-    induction xs; simpl.
-    intro. exact id.
-    intros. apply wfpf; [apply IHxs |]; wf_auto2.
+    pose proof (foldr_preserves_function t well_formed f x xs wfx).
+    simpl in H.
+    ospecialize* H.
+    apply foldr_andb_equiv_foldr_conj.
+    unfold wf in wfxs. rewrite ! foldr_map_thing in wfxs. exact wfxs.
+    exact wfpf.
+    exact H.
   Defined.
 
   Lemma mf_fold_left {A : Type} (f : Pattern -> A -> Pattern) (t : A -> Pattern) x xs :
     mu_free x ->
-    forallb mu_free (map t xs) ->
+    foldr (fun c a => mu_free c && a) true (map t xs) ->
     (forall a b, mu_free a -> mu_free (t b) -> mu_free (f a b)) ->
     mu_free (fold_left f xs x).
   Proof.
+    (* intros mfx mfxs mfpf. *)
+    (* revert x mfx mfxs. *)
+    (* induction xs; simpl. *)
+    (* now intros. *)
+    (* intros ? ? []%andb_prop. *)
+    (* apply IHxs. apply mfpf. *)
+    (* all: assumption. *)
+  (* Restart. *)
     intros mfx mfxs mfpf.
-    revert x mfx mfxs.
-    induction xs; simpl.
-    now intros.
-    intros ? ? []%andb_prop.
-    apply IHxs. apply mfpf.
-    all: assumption.
+    pose proof (fold_left_preserves_function t mu_free f x xs mfx).
+    simpl in H.
+    ospecialize* H.
+    apply foldr_andb_equiv_foldr_conj. rewrite foldr_map_thing in mfxs. exact mfxs.
+    exact mfpf.
+    exact H.
   Defined.
 
-  Lemma mf_evar_subst φ φ' x :
-    mu_free φ -> mu_free φ' ->
-    mu_free φ^[[evar: x ↦ φ']].
+  Lemma mu_free_free_evar_subst :
+    forall φ ψ x,
+    mu_free φ -> mu_free ψ ->
+    mu_free (free_evar_subst ψ x φ).
+  Proof.
+    induction φ; intros; simpl; auto.
+    * case_match; auto.
+    * rewrite IHφ1. 3: rewrite IHφ2. all: simpl in H; destruct_and! H; auto.
+    * rewrite IHφ1. 3: rewrite IHφ2. all: simpl in H; destruct_and! H; auto.
+  Qed.
+
+  (* This might change to parallel substitution *)
+  Definition substitute_list (σ : list (evar * Pattern)) (t : Pattern) : Pattern := fold_left (fun φ '(x, φ') => φ^[[evar: x ↦ φ']]) σ t.
+
+  Lemma wf_substitute_list : forall σ t, wf (map snd σ) -> well_formed t -> well_formed (substitute_list σ t).
   Proof.
     intros.
-    induction φ; simpl; try split.
-    * destruct (decide (x = x0)); auto.
-    * simpl in H. apply andb_true_iff in H as []. apply andb_true_iff. split; [exact (IHφ1 H) | exact (IHφ2 H1)].
-    * simpl in H. apply andb_true_iff in H as []. apply andb_true_iff. split; [exact (IHφ1 H) | exact (IHφ2 H1)].
-    * simpl in H. auto.
-    * inversion H.
-  Defined.
+    apply wf_fold_left with (t := snd); try assumption.
+    intros ? [] **; wf_auto2.
+  Qed.
 
-  Lemma Lemma₂_multi_right : forall Γ φ subs,
+  Definition predicate_list (σ : list (evar * Pattern)) : Pattern := fold_right (fun '(x, φ') φ => patt_free_evar x =ml φ' and φ) patt_top σ.
+
+  Lemma wf_predicate_list : forall σ, wf (map snd σ) -> well_formed (predicate_list σ).
+  Proof.
+    intros.
+    apply wf_foldr with (t := snd);
+    only 3: intros ? [] **; wf_auto2.
+  Qed.
+  
+  (* Lemma Lemma₂_half : forall Γ φ subs,
     theory ⊆ Γ -> mu_free φ -> well_formed φ ->
-    (* fold_right (fun '(_, φ') a => well_formed φ' && a) true subs -> *)
     forallb mu_free (map snd subs) -> wf (map snd subs) ->
-    Γ ⊢ fold_left (fun a '(x, φ') => a^[[evar: x ↦ φ']]) subs φ and fold_right (fun '(x, φ') a => patt_free_evar x =ml φ' and a) patt_top subs --->
-      φ and fold_right (fun '(x, φ') a => patt_free_evar x =ml φ' and a) patt_top subs.
+    Γ ⊢ substitute_list subs φ and predicate_list subs --->
+      φ and predicate_list subs.
   Proof.
     intros Γ φ subs HΓ mfφ wfφ mfs wfs.
     induction subs as [ | [x φ'] ]; simpl in * |- *.
@@ -338,7 +455,7 @@ Section ProofSystemTheorems.
       simpl.
       apply mf_fold_left with (t := snd).
       1, 2: wf_auto2.
-      intros ? [] ? ?. apply mf_evar_subst; assumption.
+      intros ? [] ? ?. apply mu_free_free_evar_subst; assumption.
     }
     cbn in H.
     rewrite free_evar_subst_id in H.
@@ -371,36 +488,54 @@ Section ProofSystemTheorems.
     mlSplitAnd.
     mlExact "H3".
     mlExact "IHspec2".
-  Abort.
+     Abort. *)
 
-  Lemma Lemma₁_meta : forall φ t x Γ, theory ⊆ Γ ->
-    well_formed φ ->
-    mu_free φ ->
-    well_formed t ->
-    Γ ⊢ (patt_free_evar x) =ml t ->
-    Γ ⊢ φ^[[evar:x↦t]] =ml φ.
+  Lemma extract_common_from_equivalence_r Γ a b c i :
+    well_formed a -> well_formed b -> well_formed c ->
+    Γ ⊢i (b and a <---> c and a) <---> (a ---> b <---> c) using i.
   Proof.
-    intros φ t x Γ HΓ WFφ MFφ WFt H.
-    pose proof (equality_elimination_basic Γ (patt_free_evar x) t {| pcEvar := x; pcPattern := φ |} HΓ ltac:(wf_auto2) WFt ltac:(wf_auto2) MFφ).
-    cbn in H0.
-    pose proof (MP H H0).
-    pose proof (pf_iff_equiv_sym_nowf Γ (φ^[[evar:x↦patt_free_evar x]]) (φ^[[evar:x↦t]]) _ H1).
-    pose proof (free_evar_subst_id φ x).
-    rewrite H3 in H2.
-    pose proof (patt_iff_implies_equal (φ^[[evar:x↦t]]) φ Γ AnyReasoning ltac:(wf_auto2) WFφ ltac:(try_solve_pile) H2).
-    exact H4.
+    intros wfa wfb wfc.
+    pose proof (extract_common_from_equivalence Γ a b c wfa wfb wfc).
+    use i in H.
+    pose proof (patt_and_comm Γ b a wfb wfa).
+    use i in H0.
+    pose proof (patt_and_comm Γ c a wfc wfa).
+    use i in H1.
+    mlRewrite H0 at 1.
+    mlRewrite H1 at 1.
+    fromMLGoal.
+    exact H.
   Defined.
 
-  Lemma mu_free_free_evar_subst :
-    forall φ ψ x,
-    mu_free φ -> mu_free ψ ->
-    mu_free (free_evar_subst ψ x φ).
+  Lemma pf_iff_equiv_trans_obj : forall Γ A B C i,
+    well_formed A -> well_formed B -> well_formed C ->
+    Γ ⊢i (A <---> B) ---> (B <---> C) ---> (A <---> C) using i.
   Proof.
-    induction φ; intros; simpl; auto.
-    * case_match; auto.
-    * rewrite IHφ1. 3: rewrite IHφ2. all: simpl in H; destruct_and! H; auto.
-    * rewrite IHφ1. 3: rewrite IHφ2. all: simpl in H; destruct_and! H; auto.
-  Qed.
+    intros * wfA wfB wfC.
+    do 2 mlIntro.
+    mlDestructAnd "0".
+    mlDestructAnd "1".
+    mlSplitAnd.
+    pose proof (syllogism Γ _ _ _ wfA wfB wfC).
+    use i in H.
+    mlApplyMeta H in "2".
+    mlApply "0" in "2".
+    mlExact "0".
+    pose proof (syllogism Γ _ _ _ wfC wfB wfA).
+    use i in H.
+    mlApplyMeta H in "4".
+    mlApply "4" in "3".
+    mlExact "3".
+  Defined.
+
+  Lemma pf_iff_equiv_sym_obj Γ A B i :
+    well_formed A -> well_formed B -> Γ ⊢i (A <---> B) ---> (B <---> A) using i.
+  Proof.
+    intros wfa wfb.
+    mlIntro.
+    mlDestructAnd "0".
+    mlSplitAnd; mlAssumption.
+  Defined.
 
   Lemma free_evar_subst_chain :
     forall φ x y ψ,
@@ -418,42 +553,721 @@ Section ProofSystemTheorems.
     * rewrite IHφ; by set_solver.
   Qed.
 
-  Lemma Lemma₁ : forall φ t x Γ, theory ⊆ Γ ->
+  Definition patt_and_wrapper : forall (a b : sig well_formed), sig well_formed.
+  Proof.
+    intros [a wfa] [b wfb].
+    exists (a and b).
+    now apply well_formed_and.
+  Defined.
+
+  Definition get_fresh_evar (φ : Pattern) : sig (.∉ free_evars φ).
+  Proof.
+    exists (fresh_evar φ); auto.
+  Defined.
+
+  Lemma Lemma₁ : forall Γ φ t x, theory ⊆ Γ ->
     well_formed φ ->
     mu_free φ ->
     well_formed t ->
     Γ ⊢ (patt_free_evar x) =ml t ---> φ^[[evar:x↦t]] =ml φ.
   Proof.
-    intros φ t x Γ HΓ WFφ MFφ WFt.
-    remember (fresh_evar φ) as y.
-    assert (mu_free (φ^[[evar:x↦patt_free_evar y]] =ml φ)) as How. {
-      cbn. rewrite mu_free_free_evar_subst; auto.
-      rewrite MFφ. reflexivity.
-    }
-    assert (Hy : y ∉ free_evars φ) by (subst y; solve_fresh).
-    pose proof (equality_elimination_basic Γ (patt_free_evar x) t {| pcEvar := y; pcPattern := φ^[[evar:x↦patt_free_evar y]] =ml φ |} HΓ ltac:(wf_auto2) WFt ltac:(wf_auto2) How).
-    Opaque "=ml".
-    cbn in H.
-    replace ((φ^[[evar:x↦patt_free_evar y]] =ml φ)^[[evar:y↦ patt_free_evar x]]) with ((φ^[[evar:x↦patt_free_evar y]]^[[evar:y↦ patt_free_evar x]] =ml φ^[[evar:y↦ patt_free_evar x]])) in H by reflexivity.
-    replace ((φ^[[evar:x↦patt_free_evar y]] =ml φ)^[[evar:y↦t]]) with ((φ^[[evar:x↦patt_free_evar y]]^[[evar:y↦t]] =ml φ^[[evar:y↦t]])) in H by reflexivity.
-    rewrite ! free_evar_subst_chain in H.
-    1-2: assumption.
-    rewrite free_evar_subst_id in H.
-    rewrite ! (free_evar_subst_no_occurrence y) in H.
-    1-2: assumption.
+    (* intros φ t x Γ HΓ WFφ MFφ WFt. *)
+    (* remember (fresh_evar φ) as y. *)
+    (* assert (mu_free (φ^[[evar:x↦patt_free_evar y]] =ml φ)) as How. { *)
+    (*   cbn. rewrite mu_free_free_evar_subst; auto. *)
+    (*   rewrite MFφ. reflexivity. *)
+    (* } *)
+    (* assert (Hy : y ∉ free_evars φ) by (subst y; solve_fresh). *)
+    (* pose proof (equality_elimination_basic Γ (patt_free_evar x) t {| pcEvar := y; pcPattern := φ^[[evar:x↦patt_free_evar y]] =ml φ |} HΓ ltac:(wf_auto2) WFt ltac:(wf_auto2) How). *)
+    (* Opaque "=ml". *)
+    (* cbn in H. *)
+    (* replace ((φ^[[evar:x↦patt_free_evar y]] =ml φ)^[[evar:y↦ patt_free_evar x]]) with ((φ^[[evar:x↦patt_free_evar y]]^[[evar:y↦ patt_free_evar x]] =ml φ^[[evar:y↦ patt_free_evar x]])) in H by reflexivity. *)
+    (* replace ((φ^[[evar:x↦patt_free_evar y]] =ml φ)^[[evar:y↦t]]) with ((φ^[[evar:x↦patt_free_evar y]]^[[evar:y↦t]] =ml φ^[[evar:y↦t]])) in H by reflexivity. *)
+    (* rewrite ! free_evar_subst_chain in H. *)
+    (* 1-2: assumption. *)
+    (* rewrite free_evar_subst_id in H. *)
+    (* rewrite ! (free_evar_subst_no_occurrence y) in H. *)
+    (* 1-2: assumption. *)
+    (* mlIntro "H". *)
+    (* mlAdd H as "H1". *)
+    (* (1* specialize? *1) *)
+    (* mlAssert ("H2" : (φ =ml φ <---> φ^[[evar:x↦t]] =ml φ)). *)
+    (* wf_auto2. *)
+    (* mlApply "H1". *)
+    (* mlExact "H". *)
+    (* (1* specialize? *1) *)
+    (* Transparent "=ml". *)
+    (* mlDestructAnd "H2" as "H3" "H4". *)
+    (* mlApply "H3". *)
+    (* mlReflexivity. *)
+  (* Restart. *)
+    intros * HΓ wfφ mfφ wft.
+    pose proof (get_fresh_evar φ) as [y Hy].
+    pose proof (equality_elimination_basic Γ (patt_free_evar x) t {| pcEvar := y; pcPattern := φ^[[evar: x ↦ patt_free_evar y]] =ml φ |}).
+    ospecialize* H; auto. wf_auto2.
+    simpl. now erewrite mu_free_free_evar_subst, mfφ.
+    cbn -["=ml"] in H. mlSimpl in H.
+    erewrite ! free_evar_subst_chain, free_evar_subst_id, ! (free_evar_subst_no_occurrence y) in H by auto.
     mlIntro "H".
-    mlAdd H as "H1".
-    (* specialize? *)
-    mlAssert ("H2" : (φ =ml φ <---> φ^[[evar:x↦t]] =ml φ)).
-    wf_auto2.
-    mlApply "H1".
-    mlExact "H".
-    (* specialize? *)
-    Transparent "=ml".
-    mlDestructAnd "H2" as "H3" "H4".
-    mlApply "H3".
-    mlReflexivity.
+    mlApplyMeta H in "H".
+    mlDestructAnd "H" as "H1" "H2".
+    mlApply "H1". mlReflexivity.
   Defined.
+
+  (* Goal forall σ φ x t, (substitute_list σ φ)^[[evar:x↦t]] = substitute_list (map (fun '(e, p) => (e, p^[[evar:x↦t]])) σ) φ^[[evar:x↦t]]. *)
+  (* Proof. *)
+  (*   intros. *)
+  (*   induction σ; simpl. *)
+  (*   reflexivity. *)
+  (*   destruct a. *)
+  (* Abort. *)
+
+  (* Goal forall σ φ x t, (forall p, In p σ -> x ∉ free_evars (snd p)) -> (x ∉ free_evars φ) -> (substitute_list σ φ)^[[evar:x↦t]] = substitute_list σ φ^[[evar:x↦t]]. *)
+  (* Proof. *)
+  (*   intros. *)
+  (*   induction σ; simpl. *)
+  (*   reflexivity. *)
+  (*   destruct a. *)
+  (* Abort. *)
+
+  (* From Coq.Arith Require Import Wf_nat. *)
+
+  Lemma Lemma₂ : forall Γ φ σ (i : ProofInfo),
+    theory ⊆ Γ -> mu_free φ -> well_formed φ ->
+    forallb mu_free (map snd σ) -> wf (map snd σ) ->
+    Γ ⊢i substitute_list σ φ and predicate_list σ <--->
+      φ and predicate_list σ using i.
+  Proof.
+    intros * HΓ mfφ wfφ mfσ wfσ.
+    pose proof (wf_predicate_list σ wfσ) as WF1.
+    pose proof (wf_substitute_list σ φ wfσ wfφ) as WF2.
+    epose proof (extract_common_from_equivalence_r _ _ _ _ _ _ _).
+    eapply (pf_iff_proj2 _ _ _ _ _ _) in H.
+    (* use i in H. *)
+    mlApplyMeta H.
+    clear H.
+    fromMLGoal.
+    generalize dependent φ.
+    (* induction σ using (induction_ltof1 _ length). intros. *)
+    induction σ; simpl; intros. mlIntro. mlReflexivity. destruct a.
+    mlIntro "H". mlDestructAnd "H" as "H1" "H2".
+    unshelve ospecialize* IHσ. exact φ^[[evar:e↦p]]. 1-6, 8: shelve.
+    mlApplyMeta IHσ in "H2". clear IHσ.
+    mlApplyMeta (pf_iff_equiv_trans_obj) in "H2".
+    mlApply "H2". mlClear "H2".
+    epose proof (Lemma₁ _ φ _ _ _ _ _ _).
+    mlApplyMeta H in "H1". clear H. 2: admit.
+    (* mlSymmetry in "H1". *)
+    (* mlRewriteBy "H1" at 1. *)
+    epose proof (get_fresh_evar (φ^[[evar:e↦p]] <---> φ)) as [y Hy].
+    epose proof (total_phi_impl_phi _ _ _ _ Hy _).
+    mlApplyMeta H in "H1". clear H.
+    (* ^ mlRewriteBy should be able to do this much ^ *)
+    mlExact "H1". admit.
+    Unshelve. all: try solve [auto | wf_auto2].
+    simpl in mfσ. apply andb_true_iff in mfσ as [].
+    apply mu_free_free_evar_subst; auto.
+  Admitted.
+
+  (* Proof. *)
+    (* unfold ltof in H. *)
+    (* destruct σ; simpl. mlIntro. mlReflexivity. *)
+    (* destruct p. *)
+    (* specialize (H σ). ospecialize* H. 1-5, 7: shelve. *)
+    (* mlIntro "H". mlDestructAnd "H" as "H1" "H2". *)
+    (* mlApplyMeta H in "H2". clear H. *)
+    (* epose proof (Lemma₁ φ _ _ _ _ _ _ _ ). *)
+    (* mlApplyMeta H in "H1". clear H. 2: admit. *)
+    (* epose proof (pf_iff_equiv_trans_obj _ (substitute_list σ φ^[[evar:e↦p]]) _ φ _ _ _ _). *)
+    (* mlAssert ("H0" : (substitute_list σ φ^[[evar:e↦p]] <---> substitute_list σ φ)). *)
+    (* shelve. clear Hwf. *)
+    (* Fail mlRewriteBy "H1" at 1. *)
+
+
+    (* induction σ; simpl. *)
+    (* mlIntro. mlReflexivity. *)
+    (* destruct a. *)
+    (* ospecialize* IHσ. 1-4, 6: shelve. *)
+    (* mlIntro "H". *)
+    (* mlDestructAnd "H" as "H1" "H2". *)
+    (* mlApplyMeta IHσ in "H2". clear IHσ. *)
+    (* epose proof (Lemma₁ φ _ _ _ _ _ _ _). *)
+    (* mlApplyMeta H in "H1". clear H. 2: admit. *)
+    (* Fail mlRewriteBy "H1" at 1. *)
+    (* evar (y : evar). *)
+    (* epose proof (equality_elimination_basic _ _ _ {| pcEvar := y; pcPattern := substitute_list σ (patt_free_evar y) |}). cbn in H. *)
+    (* ospecialize* H. 1-5: shelve. *)
+    (* mlApplyMeta H in "H1". clear H. *)
+    (* replace ((substitute_list σ (patt_free_evar y))^[[evar:y↦φ^[[evar:e↦p]]]]) with (substitute_list σ φ^[[evar:e↦p]]). *)
+    (* replace ((substitute_list σ (patt_free_evar y))^[[evar:y↦φ]]) with (substitute_list σ φ). *)
+    (* epose proof (pf_iff_equiv_trans_obj _ _ _ _ _ _ _ _). *)
+    (* mlApplyMeta H in "H1". clear H. *)
+    (* mlApply "H1" in "H2". *)
+    (* mlExact "H2". *)
+    (* transitivity (substitute_list (map (^[[evar:y↦φ]]) σ) (patt_free_evar y)^[[evar:y↦φ]]). *)
+    (* (1* generalize dependent φ. vagy induction σ using list_length_ind. *1) *)
+    (* generalize dependent φ. *)
+    (* induction σ; simpl; intros. *)
+    (* mlIntro. mlReflexivity. *)
+    (* destruct a. *)
+    (* unshelve ospecialize* IHσ. exact (φ^[[evar: e ↦ p]]). 1-6, 8: shelve. *)
+    (* mlIntro "H". mlDestructAnd "H" as "H1" "H2". *)
+    (* Fail mlRewriteBy "H1" at 1. *)
+    (* mlApplyMeta IHσ in "H2". clear IHσ. *)
+    (* (1* Undo 3. *1) *)
+    (* epose proof (equality_elimination_basic _ _ _ ({| pcEvar := e; pcPattern := substitute_list σ φ |}) HΓ _ _ _ _). cbn in H. *)
+    (* (1* mlIntro "H". mlDestructAnd "H" as "H1" "H2". *1) *)
+    (* mlApplyMeta H in "H1". clear H. *)
+    (* 2: admit. *)
+    (* rewrite free_evar_subst_id. *)
+    (* (1* emlApplyMeta (pf_iff_equiv_sym_obj _ _ _ _ _ _) in "H1". *1) *)
+    (* epose proof (pf_iff_equiv_sym_obj _ _ _ _ _ _). *)
+    (* mlApplyMeta H in "H1". clear H. *)
+    (* epose proof (pf_iff_equiv_trans_obj _ _ _ _ _ _ _ _). *)
+    (* mlApplyMeta H in "H1". clear H. *)
+    (* mlApply "H1" in "H2". mlClear "H1". *)
+    (* replace ((substitute_list σ φ)^[[evar:e↦p]]) with (substitute_list σ φ^[[evar:e↦p]]). mlExact "H2". *)
+    (* admit. *)
+    (* Unshelve. all: try solve [wf_auto2]. all: epose proof (wf_substitute_list σ φ _ _); try solve [wf_auto2]. *)
+    (* simpl. apply mf_fold_left with (t := snd). exact mfφ. *)
+    (* clear wfφ wfσ WF1 WF2 IHσ H. simpl in mfσ. *)
+    (* apply andb_true_iff in mfσ. destruct mfσ. clear H. *)
+    (* induction σ. split. *)
+    (* simpl in H0. apply andb_true_iff in H0. destruct H0. *)
+    (* specialize (IHσ H0). simpl. apply andb_true_iff. now split. *)
+    (* intros ? [] ? ?. apply mu_free_free_evar_subst; auto. *)
+    (* Unshelve. all: wf_auto2. *)
+
+  (* Admitted. *)
+
+  Definition is_unifier_of (σ : list (evar * Pattern)) t₁ t₂ := substitute_list σ t₁ =ml substitute_list σ t₂.
+
+  Lemma wf_is_unifier_of : forall σ t₁ t₂, wf (map snd σ) -> well_formed t₁ -> well_formed t₂ -> well_formed (is_unifier_of σ t₁ t₂).
+  Proof.
+    intros.
+    apply well_formed_equal; apply wf_substitute_list; assumption.
+  Qed.
+
+  Lemma patt_free_evar_subst : forall x φ, (patt_free_evar x)^[[evar: x ↦ φ]] = φ.
+  Proof.
+    intros.
+    simpl.
+    case_match.
+    reflexivity.
+    contradiction.
+  Defined.
+
+  (* Goal forall a b x Γ, theory ⊆ Γ ->
+    well_formed a -> well_formed b -> well_formed x -> mu_free x ->
+    Γ ⊢ x ---> a =ml b <---> (a and x) =ml (b and x).
+  Proof.
+    intros ? ? ? ? HΓ wfa wfb wfx mfx.
+    mlIntro "H".
+    unfold patt_iff.
+    mlSplitAnd.
+    mlIntro "H1".
+    (* remember (fresh_evar x) as y. *)
+    (* pose proof (equality_elimination_basic Γ a b {| pcEvar := y ; pcPattern := patt_free_evar y and x |} HΓ wfa wfb ltac:(wf_auto2) ltac:(wf_auto2)). *)
+    (* Opaque "and". *)
+    (* cbn in H. *)
+    (* Transparent "and". *)
+    (* mlSimpl in H. *)
+    (* rewrite ! patt_free_evar_subst in H. *)
+    (* rewrite ! free_evar_subst_no_occurrence in H; auto. *)
+    (* mlAdd H as "H2". *)
+    (* mlAssert ("H2spec" : (a and x <---> b and x)). *)
+    (* wf_auto2. *)
+    (* mlApply "H2". *)
+    (* mlExact "H1". *)
+    mlRewriteBy "H1" at 1.
+    mlReflexivity.
+    (* pose proof (patt_iff_implies_equal (a and x) (b and x) Γ AnyReasoning ltac:(wf_auto2) ltac:(wf_auto2) (pile_any _)). *)
+    (* mlApplyMeta H0 in "H2spec". *)
+    (* mlRewriteBy "H2spec" at 0. *)
+    mlIntro "H1".
+    mlSwap "H" with "H1".
+    mlDeduct "H1".
+    remember (_ : ProofInfo) as i.
+    pose proof (extract_common_from_equivalence Γ x a b wfx wfa wfb).
+    assert (Γ ∪ {[a and x <---> b and x]} ⊢i (x ---> a <---> b) using i).
+    admit.
+    assert (Γ ∪ {[a and x <---> b and x]} ⊢i (x ---> a =ml b) using i).
+    (* pose proof (hypothesis (Γ ∪ {[a and x <---> b and x]}) (a and x <---> b and x) ltac:(wf_auto2) ltac:(set_solver)). *)
+    (* 2: { assert (Γ ∪ {[a and x <---> b and x]} ⊢i a <---> b using i). admit. mlRewrite H1 at 1. *)
+    (* apply (useBasicReasoning AnyReasoning) in H. *)
+    (* mlAdd H as "H2". *)
+    (* mlDestructAnd "H2" as "H3" "H4". *)
+    (* mlClear "H4". *)
+    (* unfold "=ml". *)
+     Abort. *)
+
+  (* Lemma and_of_equiv_is_equiv_obj Γ p q p' q': *)
+  (*   well_formed p -> *)
+  (*   well_formed q -> *)
+  (*   well_formed p' -> *)
+  (*   well_formed q' -> *)
+  (*   Γ ⊢i (p <---> p') ---> *)
+  (*   (q <---> q') ---> *)
+  (*   ((p and q) <---> (p' and q')) using BasicReasoning. *)
+  (* Proof. *)
+  (*   intros wfp wfq wfp' wfq'. *)
+  (*   toMLGoal. *)
+  (*   wf_auto2. *)
+  (*   mlIntro "H". *)
+  (*   mlIntro "H1". *)
+  (*   mlDestructAnd "H" as "H2" "H3". *)
+  (*   mlDestructAnd "H1" as "H4" "H5". *)
+  (*   mlSplitAnd. *)
+  (*   mlIntro "H". *)
+  (*   mlDestructAnd "H" as "H6" "H7". *)
+  (*   mlSplitAnd. *)
+  (*   mlApply "H2". *)
+  (*   mlExact "H6". *)
+  (*   mlApply "H4". *)
+  (*   mlExact "H7". *)
+  (*   mlIntro "H". *)
+  (*   mlDestructAnd "H" as "H6" "H7". *)
+  (*   mlSplitAnd. *)
+  (*   mlApply "H3". *)
+  (*   mlExact "H6". *)
+  (*   mlApply "H5". *)
+  (*   mlExact "H7". *)
+  (* Defined. *)
+
+  (* Lemma predicate_list_total Γ σ : theory ⊆ Γ -> wf (map snd σ) -> Γ ⊢i ⌊ predicate_list σ ⌋ using BasicReasoning. *)
+  (* Proof. *)
+  (*   intros HΓ wfσ. *)
+  (*   unfold predicate_list. *)
+  (*   epose proof (foldr_preserves_function_set (λ '(x, φ'), patt_free_evar x =ml φ') (λ φ, Γ ⊢i ⌊ φ ⌋ using BasicReasoning) (λ '(x, φ') (φ : Pattern), patt_free_evar x =ml φ' and φ) patt_top σ). *)
+  (*   ospecialize* X. *)
+  (*   toMLGoal. wf_auto2. *)
+  (*   mlAdd (def_propagate_not Γ patt_bott HΓ well_formed_bott). *)
+  (*   mlAdd (bott_not_defined Γ). *)
+  (*   mlDestructAnd "0". *)
+  (*   mlApply "2". *)
+  (*   mlExact "1". *)
+  (*   clear X. *)
+  (*   induction σ; split. *)
+  (*   destruct a. *)
+  (*   unfold "=ml". *)
+  (*   Search patt_total. *)
+  (*   admit. *)
+  (*   apply IHσ. wf_auto2. *)
+  (*   intros. *)
+  (*   destruct b. *)
+  (*   toMLGoal. admit. *)
+  (*   assert (well_formed (patt_free_evar e =ml p)) as Hagyjalmarbeken by admit. *)
+  (*   assert (well_formed a) as Elegleszmar by admit. *)
+  (*   mlAdd (patt_total_and Γ (patt_free_evar e =ml p) a HΓ Hagyjalmarbeken Elegleszmar). *)
+  (*   mlDestructAnd "0". *)
+  (*   mlApply "2". *)
+  (*   mlSplitAnd. *)
+  (*   mlExactMeta H0. *)
+  (*   mlExactMeta H. *)
+  (*   exact X. *)
+  (* Admitted. *)
+
+  (* This is temporary *)
+  (* Proofs will be merged later *)
+  Axiom predicate_equiv :
+    forall Γ φ,
+      theory ⊆ Γ ->
+      well_formed φ ->
+      Γ ⊢ is_predicate_pattern φ ---> φ <---> ⌊φ⌋.
+
+  Axiom predicate_imp :
+    forall Γ φ ψ,
+      Definedness_Syntax.theory ⊆ Γ ->
+      well_formed φ ->
+      well_formed ψ ->
+      Γ ⊢ is_predicate_pattern φ --->
+          is_predicate_pattern ψ --->
+          is_predicate_pattern (φ ---> ψ).
+
+  Lemma predicate_bott : forall Γ,
+    theory ⊆ Γ -> Γ ⊢ is_predicate_pattern ⊥.
+  Proof with wf_auto2.
+    intros * HΓ.
+    unfold is_predicate_pattern.
+    toMLGoal...
+    mlRight. mlReflexivity.
+  Defined.
+
+  Lemma predicate_not : forall Γ φ,
+    theory ⊆ Γ -> well_formed φ ->
+    Γ ⊢ is_predicate_pattern φ ---> is_predicate_pattern (! φ).
+  Proof.
+    intros * HΓ wfφ.
+    unfold patt_not.
+    pose proof (predicate_imp Γ φ ⊥ HΓ wfφ well_formed_bott).
+    mlIntro.
+    mlAdd (predicate_bott Γ HΓ).
+    mlRevert "1".
+    (* mlRevert "0". *)
+    fromMLGoal.
+    exact H.
+  Defined.
+
+  Lemma predicate_or : forall Γ φ₁ φ₂,
+    theory ⊆ Γ -> well_formed φ₁ -> well_formed φ₂ ->
+    Γ ⊢ is_predicate_pattern φ₁ ---> is_predicate_pattern φ₂ --->
+        is_predicate_pattern (φ₁ or φ₂).
+  Proof.
+    intros * HΓ wfφ₁ wfφ₂.
+    unfold patt_or.
+    pose proof (predicate_not Γ φ₁ HΓ wfφ₁).
+    mlIntro.
+    mlApplyMeta H in "0".
+    fromMLGoal.
+    apply predicate_imp; auto.
+  Defined.
+
+  Lemma predicate_and : forall Γ φ₁ φ₂,
+    theory ⊆ Γ -> well_formed φ₁ -> well_formed φ₂ ->
+    Γ ⊢ is_predicate_pattern φ₁ ---> is_predicate_pattern φ₂ --->
+        is_predicate_pattern (φ₁ and φ₂).
+  Proof.
+    intros * HΓ wfφ₁ wfφ₂.
+    unfold patt_and.
+    mlIntro.
+    mlIntro.
+    mlApplyMeta predicate_not in "0".
+    mlApplyMeta predicate_not in "1".
+    mlApplyMeta predicate_or in "0".
+    mlApplyMeta predicate_not.
+    mlApply "0". mlExact "1".
+    all: auto.
+  Defined.
+
+  Lemma predicate_list_predicate Γ σ : theory ⊆ Γ -> wf (map snd σ) -> Γ ⊢ is_predicate_pattern (predicate_list σ).
+  Proof with wf_auto2.
+    intros HΓ wfσ.
+    pose proof (foldr_preserves_function_set (λ '(x, φ), patt_free_evar x =ml φ) (λ φ, well_formed φ -> Γ ⊢ is_predicate_pattern φ) (λ '(x, φ') (φ : Pattern), patt_free_evar x =ml φ' and φ) patt_top σ).
+    ospecialize* X. 1-4: clear X.
+    * intro. toMLGoal... mlLeft. mlReflexivity.
+    * induction σ; split.
+      ** destruct a. intro. unfold "=ml".
+         eapply useGenericReasoning.
+         apply pile_any.
+         apply floor_is_predicate; auto...
+      ** apply IHσ...
+    * intros ? [] ? ? ?.
+      eenough (well_formed _).
+      eenough (well_formed _).
+      pose proof (predicate_and Γ _ _ HΓ H2 H3).
+      apply (MP (H0 H2)) in H4.
+      apply (MP (H H3)) in H4.
+      exact H4.
+      all: wf_auto2.
+    * apply (wf_foldr) with (t := snd); only 3: intros ? [] ? ?...
+    * exact X.
+  Defined.
+
+  (* TODO highlight this in thesis *)
+   Lemma extract_common_from_equality_r a b x Γ :
+     theory ⊆ Γ ->
+     well_formed a -> well_formed b -> well_formed x ->
+     Γ ⊢ is_predicate_pattern x --->
+         x ---> a =ml b <---> (a and x) =ml (b and x).
+   Proof.
+     intros HΓ wfa wfb wfx.
+     mlIntro "H".
+     mlIntro "H0".
+     mlSplitAnd; mlIntro "H1".
+     mlRewriteBy "H1" at 1.
+     mlReflexivity.
+     epose proof (predicate_equiv _ _ _ _).
+     mlApplyMeta H in "H".
+     mlDestructAnd "H" as "H2" "_".
+     mlApply "H2" in "H0".
+     epose proof (patt_total_and _ _ _ _ _ _).
+     apply pf_iff_proj2 in H0.
+     use AnyReasoning in H0.
+     mlConj "H1" "H0" as "H".
+     mlApplyMeta H0 in "H".
+     clear H H0. mlClear "H0". mlClear "H2". mlClear "_". mlClear "H1".
+     mlDeduct "H".
+     remember (_ : ProofInfo) as i. clear Heqi.
+     evar Pattern.
+     epose proof (hypothesis (Γ ∪ {[p]}) p _ ltac:(set_solver)). use i in H.
+     epose proof (extract_common_from_equivalence_r _ _ _ _ _ _ _ _).
+     apply (pf_iff_proj1) in H0.
+     apply lhs_from_and in H0.
+     apply (MP H) in H0.
+     mlAdd H.
+     mlRewrite H0 at 1.
+     mlReflexivity.
+     Unshelve. all: wf_auto2.
+   Defined.
+
+  Tactic Notation "mlSpecializeHyp" constr(f) "with" constr(x) := mlApply f in x; mlClear f; mlRename x into f.
+
+  (* H1 : predicate_list can be total?
+  mlConj H0 H1 
+  bring patt_and through totality with patt_total_and
+  distribute patt_and with and_of_equiv_is_equiv_obj
+  deduction theorem *)
+  Lemma Lemma₅ : forall (σ : list (evar * Pattern)) t₁ t₂ Γ,
+    theory ⊆ Γ ->
+    well_formed t₁ -> well_formed t₂ ->
+    mu_free t₁ -> mu_free t₂ ->
+    wf (map snd σ) -> forallb mu_free (map snd σ) ->
+    Γ ⊢ is_unifier_of σ t₁ t₂ ---> predicate_list σ ---> (t₁ =ml t₂).
+  Proof.
+    intros * HΓ wft₁ wft₂ mft₁ mft₂ wfσ mfσ.
+    unfold is_unifier_of.
+    epose proof (wf_predicate_list σ wfσ) as wfpl.
+    epose proof (wf_substitute_list σ t₁ wfσ wft₁) as wfsl1.
+    epose proof (wf_substitute_list σ t₂ wfσ wft₂) as wfsl2.
+    mlIntro "H".
+    mlIntro "H0".
+    epose proof (extract_common_from_equality_r _ _ _ _ _ _ _ _).
+    epose proof (predicate_list_predicate _ _ _ _).
+    apply (MP H0) in H.
+    mlApplyMeta H in "H0".
+    mlDestructAnd "H0" as "H1" "H2".
+    mlApply "H2".
+    epose proof (Lemma₂ Γ t₁ σ AnyReasoning _ _ _ _ _).
+    mlRewrite <- H1 at 1.
+    epose proof (Lemma₂ Γ t₂ σ AnyReasoning _ _ _ _ _).
+    mlRewrite <- H2 at 1.
+    mlRewriteBy "H" at 1.
+    mlReflexivity.
+    Unshelve. all: auto.
+  Defined.
+
+    (* Proof. *)
+    (* intros * HΓ wft₁ wft₂ mft₁ mft₂ wfσ mfσ. *)
+    (* pose proof (wf_substitute_list σ t₁ wfσ wft₁) as WF1. *)
+    (* pose proof (wf_substitute_list σ t₂ wfσ wft₂) as WF2. *)
+    (* pose proof (wf_predicate_list σ wfσ) as WF3. *)
+    (* pose proof (wf_is_unifier_of σ t₁ t₂ wfσ wft₁ wft₂) as WF4. *)
+    (* mlIntro "H0". *)
+    (* mlIntro "H1". *)
+    (* unfold is_unifier_of. *)
+    (* unfold "=ml" at 1. *)
+    (* mlDeduct "H0". *)
+    (* remember (ExGen := _, SVSubst := _, KT := _, AKT := _) as i. clear Heqi. *)
+    (* epose (_ <---> _). *)
+    (* epose proof (hypothesis (Γ ∪ {[p]}) p _ ltac:(set_solver)) as Hyp. *)
+    (* use i in Hyp. *)
+    (* epose proof (prf_add_assumption _ _ _ _ _ _ Hyp) as Hyp'. *)
+    (* epose proof (extract_common_from_equivalence_r _ _ _ _ _ _ _ _). *)
+    (* apply pf_iff_proj2 in H. *)
+    (* apply (MP Hyp') in H. *)
+    (* clear Hyp'. *)
+    (* epose proof (Lemma₂ (Γ ∪ {[p]}) _ _ _ ltac:(set_solver) mft₂ wft₂ mfσ wfσ). *)
+    (* epose proof (pf_iff_equiv_trans _ _ _ _ _ _ _ _ H H0). *)
+    (* clear H0. *)
+    (* epose proof (extract_common_from_equivalence_r _ _ _ _ _ _ _ _). *)
+    (* apply pf_iff_proj1 in H0. *)
+    (* apply (MP H1) in H0. *)
+    (* clear H1. *)
+    (* apply pf_iff_equiv_sym in H. *)
+    (* epose proof (Lemma₂ (Γ ∪ {[p]}) _ _ _ ltac:(set_solver) mft₁ wft₁ mfσ wfσ). *)
+    (* epose proof (pf_iff_equiv_trans _ _ _ _ _ _ _ _ H H1). *)
+    (* clear H H1. *)
+    (* epose proof (extract_common_from_equivalence_r _ _ _ _ _ _ _ _). *)
+    (* apply pf_iff_proj1 in H. *)
+    (* apply (MP H2) in H. *)
+    (* clear H2. *)
+    (* mlAdd Hyp as "Hyp". *)
+    (* mlAdd H as "H". *)
+    (* mlAdd H0 as "H0". *)
+    (* clear Hyp H H0. subst p. *)
+    (* 2-9: shelve. *)
+    (* mlAssert ("H2" : (substitute_list σ t₂ <---> t₁)). *)
+    (* shelve. mlApply "H". mlExact "H1". mlClear "H". clear Hwf. *)
+    (* mlSpecializeHyp "H0" with "H1". *)
+    (* epose proof (pf_iff_equiv_sym_obj _ _ _ _ _ _) as H. *)
+    (* mlAdd H as "H". clear H. *)
+    (* mlSpecializeHyp "H" with "H2". *)
+    (* epose proof (pf_iff_equiv_sym_obj _ _ _ _ _ _) as H. *)
+    (* mlAdd H as "H1". clear H. *)
+    (* mlSpecializeHyp "H1" with "Hyp". *)
+    (* epose proof (pf_iff_equiv_trans_obj _ _ _ (substitute_list σ t₁) _ _ _ _). *)
+    (* mlAdd H as "H2". clear H. *)
+    (* mlSpecializeHyp "H2" with "H". *)
+    (* mlSpecializeHyp "H2" with "H1". *)
+    (* epose proof (pf_iff_equiv_trans_obj _ _ _ _ _ _ _ _). *)
+    (* mlAdd H as "H". clear H. *)
+    (* mlSpecializeHyp "H" with "H2". *)
+    (* mlSpecializeHyp "H" with "H0". *)
+    (* Fail mlRewriteBy "H" at 1. *)
+    (* admit. *)
+    (* Unshelve. all: wf_auto2. *)
+    (* Restart. *)
+
+    (* mlAdd (Lemma₂ Γ t₂ σ HΓ mft₂ wft₂ mfσ wfσ) as "H2". *)
+    (* mlAdd (Lemma₂ Γ t₁ σ HΓ mft₁ wft₁ mfσ wfσ) as "H3". *)
+    (* pose proof (predicate_list_predicate Γ σ HΓ wfσ). *)
+    (* pose proof (predicate_equiv Γ (predicate_list σ) HΓ WF3). *)
+    (* pose proof (MP H0 H1). *)
+    (* mlAssert ("H2" : (⌊ predicate_list σ ⌋)). wf_auto2. *)
+    (* mlAdd H2. mlDestructAnd "0". mlApply "1". mlExact "H1". *)
+    (* mlSwap "H0" with "H2". *)
+    (* mlConj "H2" "H0" as "H3". unfold "=ml" at 1. *)
+    (* pose proof (well_formed_iff _ _ WF1 WF2) as WF5. *)
+    (* pose proof (patt_total_and Γ _ _ HΓ WF3 WF5). *)
+    (* apply useGenericReasoning with (i := AnyReasoning) in H3. *)
+    (* 2: apply pile_any. *)
+    (* mlAdd H3. mlDestructAnd "0". mlAssert ("H4" : (⌊ predicate_list σ        and (substitute_list σ t₁ <---> substitute_list σ t₂) ⌋)). wf_auto2. mlApply "2". mlExact "H3". *)
+    (* mlClear "1". mlClear "2". mlClear "H3". mlClear "H2". *)
+    (* pose proof (and_of_equiv_is_equiv_obj Γ _ _ _ _ WF3 WF1 WF3 WF2). *)
+    (* pose proof (pf_iff_equiv_refl Γ _ WF3). *)
+    (* apply (MP H5) in H4. *)
+    (* use AnyReasoning in H4. *)
+    (* mlAdd H4. *)
+    (* mlDeduct "H4". *)
+    (* pose proof (and_of_equiv_is_equiv_obj Γ _ _ _ _  WF1 WF3 WF2 WF3). *)
+    (* use AnyReasoning in H. *)
+    (* epose proof (extract_common_from_equivalence_r Γ _ _ _ _ WF3 WF1 WF2). *)
+    (* mlAdd H. mlDestructAnd "0" as "x" "H2". clear H. mlClear "x". *)
+    (* epose proof (extract_common_from_equivalence_r Γ _ _ _ _ WF3 WF1 wft₂). *)
+    (* mlAdd H. mlDestructAnd "0" as "H2'" "x". clear H. mlClear "x". *)
+    (* epose proof (extract_common_from_equivalence_r Γ _ _ _ _ WF3 WF2 wft₁). *)
+    (* mlAdd H. mlDestructAnd "0" as "H2''" "x". clear H. mlClear "x". *)
+    (* (1* epose proof (and_of_equiv_is_equiv_obj' _ _ _ _ _ _ WF1 WF3 wft₂ WF3). *1) *)
+    (* (1* use AnyReasoning in H. *1) *)
+    (* (1* mlAdd H as "H2'". clear H. *1) *)
+    (* pose proof (pf_iff_equiv_refl Γ _ WF3). *)
+    (* use AnyReasoning in H. *)
+    (* mlAdd H as "H3". clear H. *)
+    (* epose proof (pf_iff_equiv_trans_obj Γ (substitute_list σ t₂ and predicate_list σ) (substitute_list σ t₁ and predicate_list σ) _ _ _ _ _). *)
+    (* mlAdd H as "H4". clear H. *)
+    (* epose proof (pf_iff_equiv_trans_obj Γ _ _ (t₁ and predicate_list σ) _ _ _ _). *)
+    (* mlAdd H as "H4'". clear H. *)
+    (* epose proof (pf_iff_equiv_trans_obj Γ (substitute_list σ t₁) (substitute_list σ t₂) _ _ _ _ _). *)
+    (* mlAdd H as "H4''". clear H. *)
+    (* epose proof (pf_iff_equiv_trans_obj Γ _ _ _ _ _ _ _). *)
+    (* mlAdd H as "H4'''". clear H. *)
+    (* epose proof (pf_iff_equiv_sym_obj _ (substitute_list σ t₁ and predicate_list σ) (substitute_list σ t₂ and predicate_list σ) _ _ _). *)
+    (* mlAdd H as "H5". clear H. *)
+    (* epose proof (pf_iff_equiv_sym_obj _ _ _ _ _ _). *)
+    (* mlAdd H as "H5'". clear H. *)
+    (* epose proof (pf_iff_equiv_sym_obj _ (substitute_list σ t₁) (substitute_list σ t₂) _ _ _). *)
+    (* mlAdd H as "H5'". clear H. *)
+    (* clear H0 H1 H2 H3 H4 H5 Hwf Hwf0 WF5. *)
+    (* evar Pattern. *)
+    (* enough (well_formed p) as wfp. *)
+    (* pose proof (hypothesis (Γ∪ {[predicate_list σ and (substitute_list σ t₁ <---> substitute_list σ t₂)]}) (predicate_list σ and (substitute_list σ t₁ <---> substitute_list σ t₂)) ltac:(wf_auto2) ltac:(set_solver)) as Hyp. *)
+    (* epose proof (prf_add_assumption _ _ _ _ WF3 _ Hyp). *)
+    (* mlAdd Hyp' as "Hyp'". *)
+    (* subst p. *)
+
+    (* epose proof (pf_iff_proj2 _ _ _ _ _ _ H0). *)
+    (* pose proof (MP H H1). *)
+    (* mlAdd H2 as "H4". mlAdd H2 as "H5". *)
+    (* clear Hyp H H0 H1. *)
+
+    (* pose proof (MP H2 H). *)
+    (* clear H. *)
+    (* epose proof (pf_iff_equiv_trans_obj _ _ _ _ _ _ _ _). *)
+    (* pose proof (MP H (MP H0 H3)). *)
+    (* epose proof (pf_iff_equiv_trans_obj _ _ _ _ _ _ _ _). *)
+
+    (* mlAdd H. clear H. mlDestructAnd "0" as "x" "H4". mlClear "x". *)
+    (* mlSpecializeHyp "H4" with "Hyp'". *)
+    (* subst p. *)
+    (* mlAdd Hyp. *)
+    (* mlDestructAnd "1". *)
+    (* 2: wf_auto2. *)
+    (* unfold patt_iff at 3, patt_and at 1, patt_not at 3. *)
+    (* mlApply "H2" in "Hyp'". mlClear "H2". *)
+    (* mlApply "Hyp'" in "H3". mlClear "Hyp'". *)
+    (* mlApply "H5" in "Hyp'". mlClear "H5". *)
+    (* mlAssert ("H3'" : (substitute_list σ t₂ and predicate_list σ <--->       substitute_list σ t₁ and predicate_list σ)). shelve. *)
+    (* mlApply "H5". mlExact "H3". mlClear "H5". *)
+    (* mlApply "H4" in "Hyp'". mlClear "H4". *)
+    (* mlApply "Hyp'" in "H'". mlClear "Hyp'". *)
+    (* mlApply "H5'" in "H'". mlClear "H5'". *)
+    (* mlApply "H4'''" in "H'". mlClear "H4'''". *)
+    (* mlApply "H'" in "H". mlClear "H'". *)
+    (* epose proof (extract_common_from_equivalence_r _ _ _ _ _ _ _ _). *)
+    (* mlAdd H. clear H. *)
+    (* mlDestructAnd "0" as "H2" "x". mlClear "x". *)
+    (* mlApply "H2" in "H". mlApply "H" in "H1". *)
+
+    (* mlApply "H4'" in "H3'". mlClear "H4'". *)
+    (* mlApply "H3" in "H". mlClear "H3". *)
+    (* mlApply "H3'" in "H'". mlClear "H3'". *)
+    (* mlApply "H2'" in "H". mlClear "H2'". *)
+    (* mlApply "H2''" in "H'". mlClear "H2''". *)
+    (* mlAssert ("H2" : (substitute_list σ t₁ <---> t₂)). shelve. *)
+    (* mlApply "H". mlExact "H1". mlClear "H". *)
+    (* mlApply "H'" in "H1". mlClear "H'". *)
+    (* mlApply "H4''" in "Hyp'". mlClear "H4''". *)
+    (* mlApply "Hyp'" in "H1". mlClear "Hyp'". *)
+    (* mlApply "H5'" in "H1". mlClear "H5'". *)
+    (* mlApply "H4'''" in "H1". mlClear "H4'''". *)
+    (* mlApply "H1" in "H2". mlClear "H1". *)
+    
+    (* epose proof (foldr_preserves_function_set snd (fun φ => Γ ⊢i ⌊ φ ⌋ using BasicReasoning) (λ '(x, φ') (φ : Pattern), patt_free_evar x =ml φ' and φ) Top σ). *)
+    (* simpl in X. *)
+    (* ospecialize* X. *)
+    (* toMLGoal. wf_auto2. *)
+    (* mlAdd (def_propagate_not Γ patt_bott HΓ ltac:(wf_auto2)). *)
+    (* mlAdd (bott_not_defined Γ). *)
+    (* mlDestructAnd "0". *)
+    (* mlApply "2". *)
+    (* mlExact "1". *)
+    (* (1* Search derives_using patt_and patt_total. *1) *)
+    (* (1* Search derives_using patt_iff patt_and. *1) *)
+    (* pose proof (extract_common_from_equivalence Γ (predicate_list σ) (substitute_list σ t₁) t₁). *)
+    (* ospecialize* H0. *)
+    (* apply wf_foldr with (t := snd). *)
+    (* 4: apply wf_fold_left with (t := snd). *)
+    (* 3, 6: intros ? [] ? ?. *)
+    (* 1-7: wf_auto2. *)
+    (* apply (useBasicReasoning AnyReasoning) in H0. *)
+    (* mlAdd H0 as "H2". *)
+    (* mlDestructAnd "H2" as "H3" "H4". *)
+    (* mlClear "H4". *)
+    (* mlAssert ("H3spec" : (predicate_list σ ---> substitute_list σ t₁ <---> t₁)). *)
+    (* { *)
+    (*   apply well_formed_imp. *)
+    (*   apply wf_foldr with (t := snd). *)
+    (*   4: apply well_formed_iff. *)
+    (*   4: apply wf_fold_left with (t := snd). *)
+    (*   3, 6: intros ? [] ? ?. *)
+    (*   all: wf_auto2. *)
+    (* } *)
+    (* mlApply "H3". *)
+    (* mlSplitAnd. *)
+    (* Admitted. *)
+
+  (* Lemma Lemma₅_meta : forall (σ : list (evar * Pattern)) t₁ t₂ Γ, *)
+  (*   theory ⊆ Γ -> well_formed t₁ -> well_formed t₂ -> wf (map snd σ) -> *)
+  (*   Γ ⊢ is_unifier_of σ t₁ t₂ -> Γ ⊢ predicate_list σ ---> (t₁ =ml t₂). *)
+  (* Proof. *)
+  (*   intros ? ? ? ? HΓ wft₁ wft₂ wfσ isunif. *)
+  (*   toMLGoal. *)
+  (*   { *)
+  (*     simpl. *)
+  (*     apply well_formed_imp. *)
+  (*     apply wf_foldr with (t := snd). *)
+  (*     3: intros ? [] ? ?. *)
+  (*     all: wf_auto2. *)
+  (*   } *)
+  (*   mlIntro "H". *)
+
+  (* Lemma Lemma₁_meta : forall φ t x Γ, theory ⊆ Γ ->
+    well_formed φ ->
+    mu_free φ ->
+    well_formed t ->
+    Γ ⊢ (patt_free_evar x) =ml t ->
+    Γ ⊢ φ^[[evar:x↦t]] =ml φ.
+  Proof.
+    intros φ t x Γ HΓ WFφ MFφ WFt H.
+    pose proof (equality_elimination_basic Γ (patt_free_evar x) t {| pcEvar := x; pcPattern := φ |} HΓ ltac:(wf_auto2) WFt ltac:(wf_auto2) MFφ).
+    cbn in H0.
+    pose proof (MP H H0).
+    pose proof (pf_iff_equiv_sym_nowf Γ (φ^[[evar:x↦patt_free_evar x]]) (φ^[[evar:x↦t]]) _ H1).
+    pose proof (free_evar_subst_id φ x).
+    rewrite H3 in H2.
+    pose proof (patt_iff_implies_equal (φ^[[evar:x↦t]]) φ Γ AnyReasoning ltac:(wf_auto2) WFφ ltac:(try_solve_pile) H2).
+    exact H4.
+     Defined. *)
 
   Lemma R₅' : forall x Γ, theory ⊆ Γ -> Γ ⊢ (ex , patt_free_evar x =ml b0).
   Proof.
@@ -567,6 +1381,7 @@ Section UnificationProcedure.
   Definition in_solved_form (P : unification_problem) : bool := from_option (forallb (uncurry is_free_evar_in)) true P.
 
 
+  (* fin_set gset gmap.v *)
 
 
 
